user 3, session 10289, part 14

diffs-w-failures/3/user-3-session-10289.v
@@ -103,8 +103,9 @@ Timeout 1 Check @mark.
 Set Printing Width 78.
 Unset Silent.
 Set Diffs "off".
+Unset Silent.
+Set Diffs "off".
 Set Printing Width 78.
-Hint Resolve mark: core.
 Theorem proc_spec_rx :
   forall `(spec : Specification A T R State) `(p : proc T) 
     `(rec : proc R) `(rx : T -> proc T')
@@ -116,9 +117,10 @@ Theorem proc_spec_rx :
      pre (spec a state) /\
      (forall r state',
       recovered (spec a state) r state' ->
-      Marker "recovered condition" -> recovered (spec' a' state) r state') /\
+      forall L : Marker "recovered condition",
+      recovered (spec' a' state) r state') /\
      (forall r,
-      Marker "post condition" ->
+      forall L : Marker "post condition",
       proc_spec
         (fun (_ : unit) state' =>
          {|
@@ -126,10 +128,10 @@ Theorem proc_spec_rx :
          post := fun r state'' => post (spec' a' state) r state'';
          recovered := fun r state'' => recovered (spec' a' state) r state'' |})
         (rx r) rec abs)) -> proc_spec spec' (Bind p rx) rec abs.
+Set Silent.
 Proof.
 (unfold proc_spec at 3; intros).
 inv_rexec.
-Set Silent.
 -
 inv_exec.
 (match goal with
@@ -177,5 +179,201 @@ inv_exec.
  end).
 (eapply H0 in H2; repeat deex).
 (eapply H in H10; simpl in *; safe_intuition repeat deex; eauto).
+Unset Silent.
+Qed.
+Set Silent.
+Theorem spec_intros :
+  forall `(spec : Specification A T R State) `(p : proc T) 
+    `(rec : proc R) `(abs : Abstraction State),
+  (forall a state0,
+   pre (spec a state0) ->
+   proc_spec
+     (fun (_ : unit) state =>
+      {|
+      pre := state = state0;
+      post := fun r state' => post (spec a state) r state';
+      recovered := fun r state' => recovered (spec a state) r state' |}) p
+     rec abs) -> proc_spec spec p rec abs.
+Proof.
+(unfold proc_spec at 2; intros).
+(apply H in H1).
+(eapply H1 in H2; eauto).
+(simpl in *; eauto).
+Qed.
+Ltac spec_intros := intros; eapply spec_intros; intros.
+Ltac
+ spec_case pf :=
+  eapply proc_spec_weaken; [ solve [ apply pf ] | unfold spec_impl ].
+Theorem spec_exec_equiv :
+  forall `(spec : Specification A T R State) (p p' : proc T) 
+    `(rec : proc R) `(abs : Abstraction State),
+  exec_equiv p p' -> proc_spec spec p' rec abs -> proc_spec spec p rec abs.
+Proof.
+(unfold proc_spec; intros).
+(eapply H0; eauto).
+(eapply rexec_equiv; eauto).
+(symmetry; auto).
+Qed.
+Definition rec_wipe `(rec : proc R) `(abs : Abstraction State)
+  (wipe : State -> State -> Prop) :=
+  forall T (v : T),
+  proc_spec
+    (fun (_ : unit) state =>
+     {|
+     pre := True;
+     post := fun r state' => r = v /\ state' = state;
+     recovered := fun _ state' => wipe state state' |}) 
+    (Ret v) rec abs.
+Theorem ret_spec :
+  forall `(abs : Abstraction State) (wipe : State -> State -> Prop)
+    `(spec : Specification A T R State) (v : T) (rec : proc R),
+  rec_wipe rec abs wipe ->
+  (forall a state,
+   pre (spec a state) ->
+   post (spec a state) v state /\
+   (forall state',
+    wipe state state' -> forall r, recovered (spec a state) r state')) ->
+  proc_spec spec (Ret v) rec abs.
+Proof.
+(intros).
+(unfold proc_spec; intros).
+(eapply H in H3; simpl in *; eauto).
+(eapply H0 in H2).
+(destruct r; safe_intuition repeat deex; eauto).
+Qed.
+Ltac
+ monad_simpl :=
+  repeat
+   match goal with
+   | |- proc_spec _ (Bind (Ret _) _) _ _ =>
+         eapply spec_exec_equiv; [ apply monad_left_id |  ]
+   | |- proc_spec _ (Bind (Bind _ _) _) _ _ =>
+         eapply spec_exec_equiv; [ apply monad_assoc |  ]
+   end.
+Ltac
+ step_proc_basic :=
+  match goal with
+  | |- forall _, _ => intros; step_proc_basic
+  | |- proc_spec _ (Ret _) _ _ => eapply ret_spec
+  | |- proc_spec _ _ _ _ =>
+        monad_simpl; eapply proc_spec_rx; [ solve [ eauto ] |  ]
+  | H:proc_spec _ ?p _ _
+    |- proc_spec _ ?p _ _ =>
+        eapply proc_spec_weaken; [ eapply H | unfold spec_impl ]
+  | |- proc_spec _ _ _ _ =>
+        eapply proc_spec_weaken; [ solve [ eauto ] | unfold spec_impl ]
+  end.
+Ltac
+ simplify :=
+  simpl; cbn[pre post recovered] in *;
+   repeat
+    match goal with
+    | H:_ /\ _ |- _ => destruct H
+    | |- rec_wipe _ _ _ => eauto
+    | |- forall _, _ => intros
+    | |- exists _ : unit, _ => exists tt
+    | |- _ /\ _ => split; [ solve [ trivial ] |  ]
+    | |- _ /\ _ => split; [  | solve [ trivial ] ]
+    | _ => solve [ trivial ]
+    | _ => progress subst
+    | _ => progress autounfold in *
+    end.
+Ltac step_proc := step_proc_basic; intros; simplify.
+Inductive InitResult :=
+  | Initialized : _
+  | InitFailed : _.
+Definition then_init (init1 init2 : proc InitResult) : 
+  proc InitResult :=
+  r <- init1; match r with
+              | Initialized => init2
+              | Failed => Ret Failed
+              end.
+Definition inited_any `(s : State) : Prop := True.
+Definition init_abstraction (init : proc InitResult) 
+  (rec : proc unit) `(abs : Abstraction State) (init_sem : State -> Prop) :=
+  proc_spec
+    (fun (_ : unit) w =>
+     {|
+     pre := True;
+     post := fun r w' =>
+             match r with
+             | Initialized =>
+                 exists state, abstraction abs w' state /\ init_sem state
+             | InitFailed => True
+             end;
+     recovered := fun _ w' => True |}) init rec (IdAbstraction world).
+Theorem init_abstraction_any_rec :
+  forall (init : proc InitResult) (rec rec' : proc unit)
+    `(abs : Abstraction State) (init_sem : State -> Prop),
+  init_abstraction init rec abs init_sem ->
+  init_abstraction init rec' abs init_sem.
+Proof.
+(unfold init_abstraction, proc_spec; simpl; intros).
+(destruct matches; subst; eauto).
+(eapply rexec_finish_any_rec in H2).
+(eapply H in H2; eauto).
+Qed.
+Theorem then_init_compose :
+  forall (init1 init2 : proc InitResult) (rec rec' : proc unit)
+    `(abs1 : Abstraction State1) `(abs2 : LayerAbstraction State1 State2)
+    (init1_sem : State1 -> Prop) (init2_sem : State2 -> Prop),
+  init_abstraction init1 rec abs1 init1_sem ->
+  proc_spec
+    (fun (_ : unit) state =>
+     {|
+     pre := init1_sem state;
+     post := fun r state' =>
+             match r with
+             | Initialized =>
+                 exists state'',
+                   abstraction abs2 state' state'' /\ init2_sem state''
+             | InitFailed => True
+             end;
+     recovered := fun _ state' => True |}) init2 rec abs1 ->
+  init_abstraction (then_init init1 init2) rec'
+    (abstraction_compose abs1 abs2) init2_sem.
+Proof.
+(intros).
+(eapply init_abstraction_any_rec with rec).
+(unfold init_abstraction; intros).
+(step_proc; intuition; simpl in *).
+(descend; intuition eauto).
+(destruct r).
+-
+clear H.
+(unfold proc_spec in *; intuition eauto; simpl in *; subst; repeat deex).
+(eapply H0 in H2; eauto).
+(destruct matches in *; safe_intuition repeat deex; eauto).
+(descend; intuition eauto).
+-
+(unfold proc_spec; simpl; intros).
+(destruct matches; subst; eauto).
+(eexists; intuition eauto).
+(inv_rexec; inv_exec).
+congruence.
+Qed.
+Theorem spec_abstraction_compose :
+  forall `(spec : Specification A T R State2) `(p : proc T) 
+    `(rec : proc R) `(abs2 : LayerAbstraction State1 State2)
+    `(abs1 : Abstraction State1),
+  proc_spec
+    (fun '(a, state2) state =>
+     {|
+     pre := pre (spec a state2) /\ abstraction abs2 state state2;
+     post := fun v state' =>
+             exists state2',
+               post (spec a state2) v state2' /\
+               abstraction abs2 state' state2';
+     recovered := fun v state' =>
+                  exists state2',
+                    recovered (spec a state2) v state2' /\
+                    abstraction abs2 state' state2' |}) p rec abs1 ->
+  proc_spec spec p rec (abstraction_compose abs1 abs2).
+Proof.
+(intros).
+(unfold proc_spec, abstraction_compose; simpl; intros; safe_intuition
+  repeat deex).
+(eapply (H (a, state)) in H2; simpl in *; eauto).
+(destruct r; intuition repeat deex; eauto).
 Unset Silent.
 Qed.
